coq/coq/syntax_ott.v
@@ -34,11 +34,11 @@ Inductive texp : Set :=  (*r target term *)
  | texp_proj (t1:texp) (l:label) (*r projection *)
  | texp_concat (t1:texp) (t2:texp) (*r concatenation *).
 
+Definition tctx : Set := list ( atom * ttyp ).
+
 Inductive dirflag : Set :=  (*r checking direction *)
  | Inf : dirflag
  | Chk : dirflag.
-
-Definition tctx : Set := list ( atom * ttyp ).
 
 Inductive exp : Set :=  (*r expressions *)
  | exp_top : exp (*r top value *)
@@ -63,7 +63,7 @@ Definition ctx : Set := list ( atom * typ ).
 (** opening up abstractions *)
 Fixpoint open_texp_wrt_texp_rec (k:nat) (t_5:texp) (t__6:texp) {struct t__6}: texp :=
   match t__6 with
-  | (texp_var_b nat) => 
+  | (texp_var_b nat) =>
       match lt_eq_lt_dec nat k with
         | inleft (left _) => texp_var_b nat
         | inleft (right _) => t_5
@@ -74,7 +74,7 @@ Fixpoint open_texp_wrt_texp_rec (k:nat) (t_5:texp) (t__6:texp) {struct t__6}: te
   | (texp_abs t) => texp_abs (open_texp_wrt_texp_rec (S k) t_5 t)
   | (texp_fixpoint t) => texp_fixpoint (open_texp_wrt_texp_rec (S k) t_5 t)
   | (texp_app t1 t2) => texp_app (open_texp_wrt_texp_rec k t_5 t1) (open_texp_wrt_texp_rec k t_5 t2)
-  | texp_nil => texp_nil 
+  | texp_nil => texp_nil
   | (texp_cons l t1' t2) => texp_cons l (open_texp_wrt_texp_rec k t_5 t1') (open_texp_wrt_texp_rec k t_5 t2)
   | (texp_proj t1 l) => texp_proj (open_texp_wrt_texp_rec k t_5 t1) l
   | (texp_concat t1 t2) => texp_concat (open_texp_wrt_texp_rec k t_5 t1) (open_texp_wrt_texp_rec k t_5 t2)
@@ -82,9 +82,9 @@ end.
 
 Fixpoint open_exp_wrt_exp_rec (k:nat) (e_5:exp) (e__6:exp) {struct e__6}: exp :=
   match e__6 with
-  | exp_top => exp_top 
+  | exp_top => exp_top
   | (exp_base b) => exp_base b
-  | (exp_var_b nat) => 
+  | (exp_var_b nat) =>
       match lt_eq_lt_dec nat k with
         | inleft (left _) => exp_var_b nat
         | inleft (right _) => e_5
@@ -123,7 +123,7 @@ Inductive lc_texp : texp -> Prop :=    (* defn lc_texp *)
      (lc_texp t1) ->
      (lc_texp t2) ->
      (lc_texp (texp_app t1 t2))
- | lc_texp_nil : 
+ | lc_texp_nil :
      (lc_texp texp_nil)
  | lc_texp_cons : forall (l:label) (t1' t2:texp),
      (lc_texp t1') ->
@@ -139,7 +139,7 @@ Inductive lc_texp : texp -> Prop :=    (* defn lc_texp *)
 
 (* defns LC_exp *)
 Inductive lc_exp : exp -> Prop :=    (* defn lc_exp *)
- | lc_exp_top : 
+ | lc_exp_top :
      (lc_exp exp_top)
  | lc_exp_base : forall (b:lit),
      (lc_exp (exp_base b))
@@ -201,7 +201,7 @@ end.
 (** substitutions *)
 Fixpoint esubst_exp (e_5:exp) (x5:var) (e__6:exp) {struct e__6} : exp :=
   match e__6 with
-  | exp_top => exp_top 
+  | exp_top => exp_top
   | (exp_base b) => exp_base b
   | (exp_var_b nat) => exp_var_b nat
   | (exp_var_f x) => (if eq_var x x5 then e_5 else (exp_var_f x))
@@ -222,7 +222,7 @@ Fixpoint subst_texp (t_5:texp) (x5:var) (t__6:texp) {struct t__6} : texp :=
   | (texp_abs t) => texp_abs (subst_texp t_5 x5 t)
   | (texp_fixpoint t) => texp_fixpoint (subst_texp t_5 x5 t)
   | (texp_app t1 t2) => texp_app (subst_texp t_5 x5 t1) (subst_texp t_5 x5 t2)
-  | texp_nil => texp_nil 
+  | texp_nil => texp_nil
   | (texp_cons l t1' t2) => texp_cons l (subst_texp t_5 x5 t1') (subst_texp t_5 x5 t2)
   | (texp_proj t1 l) => texp_proj (subst_texp t_5 x5 t1) l
   | (texp_concat t1 t2) => texp_concat (subst_texp t_5 x5 t1) (subst_texp t_5 x5 t2)
@@ -269,7 +269,7 @@ Fixpoint stype2string (A: typ) : LS :=
     | typ_rcd l A' => ["{" ++  l ++ "=>" ++ (stype2string A') ++ "}"]
     | typ_and A1 A2 => nodup string_dec (merge (stype2string A1) (stype2string A2))
     end.
-    
+
 Notation "|| A ||" := (stype2string A) (at level 50, A at next level). (* 1 is too high *)
 
 Fixpoint ttyp_concat_simpl (A: ttyp) (B: ttyp) :=
@@ -310,11 +310,33 @@ Fixpoint Tlookup (i:string) (T:ttyp) : option ttyp :=
   end.
 
 
+(* defns RecordTypes *)
+Inductive rec_typ : ttyp -> Prop :=    (* defn rec_typ *)
+ | RT_Nil :
+     rec_typ ttyp_top
+ | RT_Rcd : forall (l:label) (At Bt:ttyp),
+     rec_typ Bt ->
+     rec_typ (ttyp_rcd l At Bt).
+
+
+Inductive subTarget : ttyp -> ttyp -> Prop :=
+ | ST_refl : forall At,
+     subTarget At At
+| ST_arrow: forall At Bt At' Bt',
+    subTarget At At' -> subTarget At' At -> subTarget Bt Bt' -> subTarget Bt' Bt -> subTarget (ttyp_arrow At Bt) (ttyp_arrow At' Bt')
+ | ST_rcd : forall At Bt,
+     rec_typ At -> rec_typ Bt ->
+     (forall l Ct, Tlookup l At = Some Ct -> exists Ct', Tlookup l Bt = Some Ct' /\ subTarget Ct' Ct /\ subTarget Ct Ct') ->
+     subTarget Bt At.
+
+#[export] Hint Constructors subTarget : core.
+
+
 (** definitions *)
 
 (* defns TopLikeType *)
 Inductive toplike : typ -> Prop :=    (* defn toplike *)
- | TL_top : 
+ | TL_top :
      toplike typ_top
  | TL_and : forall (A B:typ),
      toplike A ->
@@ -327,56 +349,22 @@ Inductive toplike : typ -> Prop :=    (* defn toplike *)
      toplike B ->
      toplike (typ_rcd l B).
 
-(* defns EqIndexType *)
-Inductive eqIndTyp : typ -> typ -> Prop :=    (* defn eqIndTyp *)
- | EI_refl : forall (A:typ),
-     eqIndTyp A A
- | EI_trans : forall (A C B:typ),
-     eqIndTyp A B ->
-     eqIndTyp B C ->
-     eqIndTyp A C
- | EI_symm : forall (A B:typ),
-     eqIndTyp B A ->
-     eqIndTyp A B
- | EI_arrow : forall (A1 B1 A2 B2:typ),
-     eqIndTyp A1 A2 ->
-     eqIndTyp B1 B2 ->
-     eqIndTyp (typ_arrow A1 B1) (typ_arrow A2 B2)
- | EI_rcd : forall (l:label) (A B:typ),
-     eqIndTyp A B ->
-     eqIndTyp (typ_rcd l A) (typ_rcd l B)
- | EI_and : forall (A B A':typ),
-     eqIndTyp A A' ->
-     eqIndTyp (typ_and A B) (typ_and A' B)
- | EI_comm : forall (A B:typ),
-     eqIndTyp (typ_and A B) (typ_and B A)
- | EI_assoc : forall (A B C:typ),
-     eqIndTyp (typ_and A  (typ_and B C) ) (typ_and  (typ_and A B)  C)
- | EI_top : forall (A:typ),
-     toplike A ->
-     eqIndTyp A typ_top
- | EI_topelim : forall (A:typ),
-     eqIndTyp (typ_and typ_top A) A
- | EI_dup : forall (A1 A2:typ),
-     eqIndTyp A1 A2 ->
-     eqIndTyp (typ_and A1 A2) A1.
-
 (* defns SplitType *)
 Inductive spl : typ -> typ -> typ -> Prop :=    (* defn spl *)
  | Sp_and : forall (A B:typ),
-     spl  (typ_and A B)   A   B 
+     spl  (typ_and A B)   A   B
  | Sp_arrow : forall (A B B1 B2:typ),
      spl B B1 B2 ->
-     spl  (typ_arrow A B)   (typ_arrow A B1)   (typ_arrow A B2) 
+     spl  (typ_arrow A B)   (typ_arrow A B1)   (typ_arrow A B2)
  | Sp_rcd : forall (l:label) (B B1 B2:typ),
      spl B B1 B2 ->
      spl (typ_rcd l B) (typ_rcd l B1) (typ_rcd l B2).
 
 (* defns OrdinaryType *)
 Inductive ord : typ -> Prop :=    (* defn ord *)
- | O_top : 
+ | O_top :
      ord typ_top
- | O_int : 
+ | O_int :
      ord typ_base
  | O_arrow : forall (A B:typ),
      ord B ->
@@ -423,15 +411,50 @@ Inductive disjoint : typ -> typ -> Prop :=    (* defn disjoint *)
 
 (* defns CoMerge *)
 Inductive comerge : texp -> typ -> typ -> texp -> typ -> texp -> Prop :=    (* defn comerge *)
+ | M_Top : forall (t1:texp) (A C:typ) (t2:texp) (B:typ),
+     lc_texp t1 ->
+     lc_texp t2 ->
+     toplike C ->
+     spl C A B ->
+     comerge t1 A C t2 B texp_nil
  | M_And : forall (t1:texp) (A B:typ) (t2:texp),
      lc_texp t1 ->
      lc_texp t2 ->
+      not ( toplike (typ_and A B) )  ->
      comerge t1 A (typ_and A B) t2 B (texp_concat t1 t2)
  | M_Arrow : forall (L:vars) (t1:texp) (A B1 B:typ) (t2:texp) (B2:typ) (t:texp),
+      not ( toplike B1 )  ->
+      not ( toplike B2 )  ->
       ( forall x , x \notin  L  -> comerge (texp_app   (texp_proj  t1  (stype2string  (typ_arrow A B1) ))   (texp_var_f x)) B1 B (texp_app   (texp_proj  t2  (stype2string  (typ_arrow A B2) ))   (texp_var_f x)) B2  ( open_texp_wrt_texp t (texp_var_f x) )  )  ->
-     comerge t1 (typ_arrow A B1) (typ_arrow A B) t2 (typ_arrow A B2)  (texp_cons (stype2string  (typ_arrow A B) )  (texp_abs t)  texp_nil) 
+     comerge t1 (typ_arrow A B1) (typ_arrow A B) t2 (typ_arrow A B2)  (texp_cons (stype2string  (typ_arrow A B) )  (texp_abs t)  texp_nil)
+ | M_ArrowL : forall (L:vars) (t1:texp) (A B1 B:typ) (t2:texp) (B2:typ) (t:texp),
+     lc_texp t2 ->
+      not ( toplike B1 )  ->
+     toplike B2 ->
+      ( forall x , x \notin  L  -> comerge (texp_app   (texp_proj  t1  (stype2string  (typ_arrow A B1) ))   (texp_var_f x)) B1 B texp_nil B2  ( open_texp_wrt_texp t (texp_var_f x) )  )  ->
+     comerge t1 (typ_arrow A B1) (typ_arrow A B) t2 (typ_arrow A B2)  (texp_cons (stype2string  (typ_arrow A B) )  (texp_abs t)  texp_nil)
+ | M_ArrowR : forall (L:vars) (t1:texp) (A B1 B:typ) (t2:texp) (B2:typ) (t:texp),
+     lc_texp t1 ->
+     toplike B1 ->
+      not ( toplike B2 )  ->
+      ( forall x , x \notin  L  -> comerge texp_nil B1 B (texp_app   (texp_proj  t2  (stype2string  (typ_arrow A B2) ))   (texp_var_f x)) B2  ( open_texp_wrt_texp t (texp_var_f x) )  )  ->
+     comerge t1 (typ_arrow A B1) (typ_arrow A B) t2 (typ_arrow A B2)  (texp_cons (stype2string  (typ_arrow A B) )  (texp_abs t)  texp_nil)
  | M_Rcd : forall (t1:texp) (l:label) (A1 A:typ) (t2:texp) (A2:typ) (t:texp),
+      not ( toplike A1 )  ->
+      not ( toplike A2 )  ->
      comerge  (texp_proj  t1  (stype2string  (typ_rcd l A1) ))  A1 A  (texp_proj  t2  (stype2string  (typ_rcd l A2) ))  A2 t ->
+     comerge t1 (typ_rcd l A1) (typ_rcd l A) t2 (typ_rcd l A2)  (texp_cons (stype2string  (typ_rcd l A) )  t  texp_nil)
+ | M_RcdL : forall (t1:texp) (l:label) (A1 A:typ) (t2:texp) (A2:typ) (t:texp),
+     lc_texp t2 ->
+      not ( toplike A1 )  ->
+     toplike A2 ->
+     comerge  (texp_proj  t1  (stype2string  (typ_rcd l A1) ))  A1 A texp_nil A2 t ->
+     comerge t1 (typ_rcd l A1) (typ_rcd l A) t2 (typ_rcd l A2)  (texp_cons (stype2string  (typ_rcd l A) )  t  texp_nil)
+ | M_RcdR : forall (t1:texp) (l:label) (A1 A:typ) (t2:texp) (A2:typ) (t:texp),
+     lc_texp t1 ->
+     toplike A1 ->
+      not ( toplike A2 )  ->
+     comerge texp_nil A1 A  (texp_proj  t2  (stype2string  (typ_rcd l A2) ))  A2 t ->
      comerge t1 (typ_rcd l A1) (typ_rcd l A) t2 (typ_rcd l A2)  (texp_cons (stype2string  (typ_rcd l A) )  t  texp_nil) .
 
 (* defns CoSubtyping *)
@@ -445,20 +468,20 @@ Inductive cosub : texp -> typ -> typ -> texp -> Prop :=    (* defn cosub *)
      lc_texp t ->
      ord B ->
       not ( toplike B )  ->
-     cosub t typ_bot B  (texp_cons (stype2string  B )  (texp_fixpoint (texp_var_b 0))  texp_nil) 
+     cosub t typ_bot B  (texp_cons (stype2string  B )  (texp_fixpoint (texp_var_b 0))  texp_nil)
  | S_Base : forall (t:texp),
      lc_texp t ->
-     cosub t typ_base typ_base  (texp_cons (stype2string  typ_base )   (texp_proj  t  (stype2string  typ_base ))   texp_nil) 
+     cosub t typ_base typ_base  (texp_cons (stype2string  typ_base )   (texp_proj  t  (stype2string  typ_base ))   texp_nil)
  | S_Arrow : forall (L:vars) (t:texp) (A1 A2 B1 B2:typ) (t2 t1:texp),
      ord B2 ->
       not ( toplike B2 )  ->
       ( forall x , x \notin  L  ->  ( cosub (texp_var_f x) B1 A1 t1  /\  cosub (texp_app   (texp_proj  t  (stype2string  (typ_arrow A1 A2) ))   t1) A2 B2  ( open_texp_wrt_texp t2 (texp_var_f x) )  )  )  ->
-     cosub t (typ_arrow A1 A2) (typ_arrow B1 B2)  (texp_cons (stype2string  (typ_arrow B1 B2) )  (texp_abs t2)  texp_nil) 
+     cosub t (typ_arrow A1 A2) (typ_arrow B1 B2)  (texp_cons (stype2string  (typ_arrow B1 B2) )  (texp_abs t2)  texp_nil)
  | S_Rcd : forall (t:texp) (l:label) (A B:typ) (t2:texp),
      ord B ->
       not ( toplike B )  ->
      cosub  (texp_proj  t  (stype2string  (typ_rcd l A) ))  A B t2 ->
-     cosub t (typ_rcd l A) (typ_rcd l B)  (texp_cons (stype2string  (typ_rcd l B) )  t2  texp_nil) 
+     cosub t (typ_rcd l A) (typ_rcd l B)  (texp_cons (stype2string  (typ_rcd l B) )  t2  texp_nil)
  | S_AndL : forall (t:texp) (A B C:typ) (t':texp),
      ord C ->
      cosub t A C t' ->
@@ -476,12 +499,12 @@ Inductive cosub : texp -> typ -> typ -> texp -> Prop :=    (* defn cosub *)
 
 (* defns Subtyping *)
 Inductive sub : typ -> typ -> Prop :=    (* defn sub *)
- | S_z : 
+ | S_z :
      sub typ_base typ_base
  | S_top : forall (A B:typ),
      toplike B ->
      sub A B
- | S_bot : 
+ | S_bot :
      sub typ_bot typ_bot
  | S_arr : forall (A1 A2 B1 B2:typ),
      sub B1 A1 ->
@@ -512,9 +535,11 @@ Inductive proj : texp -> typ -> label -> texp -> typ -> Prop :=    (* defn proj 
      proj t1 A l texp_nil typ_top
  | P_RcdEq : forall (t:texp) (l:label) (A:typ),
      lc_texp t ->
+      not ( toplike A )  ->
      proj t (typ_rcd l A) l  (texp_proj  t  (stype2string  (typ_rcd l A) ))  A
  | P_RcdNeq : forall (t:texp) (l1:label) (A:typ) (l2:label),
      lc_texp t ->
+      not ( toplike A )  ->
       l1  <>  l2  ->
      proj t (typ_rcd l1 A) l2 texp_nil typ_top
  | P_And : forall (t1:texp) (A B:typ) (l:label) (t3 t4:texp) (A' B':typ),
@@ -531,6 +556,7 @@ Inductive distapp : texp -> typ -> texp -> typ -> texp -> typ -> Prop :=    (* d
      distapp t1 A t2 B texp_nil typ_top
  | A_Arrow : forall (t1:texp) (A B:typ) (t2:texp) (C:typ) (t3:texp),
      lc_texp t1 ->
+      not ( toplike B )  ->
      cosub t2 C A t3 ->
      distapp t1 (typ_arrow A B) t2 C (texp_app   (texp_proj  t1  (stype2string  (typ_arrow A B) ))   t3) B
  | A_And : forall (t1:texp) (A B:typ) (t2:texp) (C:typ) (t3 t4:texp) (A' B':typ),
@@ -554,7 +580,7 @@ Inductive elaboration : ctx -> exp -> dirflag -> typ -> texp -> Prop :=    (* de
      elaboration G (exp_rcd l e) Inf (typ_rcd l A) texp_nil
  | Ela_Base : forall (G:ctx) (b:lit),
       uniq  G  ->
-     elaboration G (exp_base b) Inf typ_base  (texp_cons (stype2string  typ_base )  (texp_base b)  texp_nil) 
+     elaboration G (exp_base b) Inf typ_base  (texp_cons (stype2string  typ_base )  (texp_base b)  texp_nil)
  | Ela_Var : forall (G:ctx) (x:var) (A:typ),
       uniq  G  ->
       binds  x A G  ->
@@ -563,16 +589,18 @@ Inductive elaboration : ctx -> exp -> dirflag -> typ -> texp -> Prop :=    (* de
       ( forall x , x \notin  L  -> elaboration  (cons ( x , A )  G )   ( open_exp_wrt_exp e (exp_var_f x) )  Chk A  ( open_texp_wrt_texp t (texp_var_f x) )  )  ->
      elaboration G (exp_fixpoint A e) Inf A (texp_fixpoint t)
  | Ela_Abs : forall (L:vars) (G:ctx) (A:typ) (e:exp) (B:typ) (t:texp),
+      not ( toplike B )  ->
       ( forall x , x \notin  L  -> elaboration  (cons ( x , A )  G )   ( open_exp_wrt_exp e (exp_var_f x) )  Chk B  ( open_texp_wrt_texp t (texp_var_f x) )  )  ->
-     elaboration G (exp_abs A e B) Inf (typ_arrow A B)  (texp_cons (stype2string  (typ_arrow A B) )  (texp_abs t)  texp_nil) 
+     elaboration G (exp_abs A e B) Inf (typ_arrow A B)  (texp_cons (stype2string  (typ_arrow A B) )  (texp_abs t)  texp_nil)
  | Ela_App : forall (G:ctx) (e1 e2:exp) (C:typ) (t3:texp) (A:typ) (t1:texp) (B':typ) (t2:texp),
      elaboration G e1 Inf A t1 ->
      elaboration G e2 Inf B' t2 ->
      distapp t1 A t2 B' t3 C ->
      elaboration G (exp_app e1 e2) Inf C t3
  | Ela_Rcd : forall (G:ctx) (l:label) (e:exp) (A:typ) (t:texp),
+      not ( toplike A )  ->
      elaboration G e Inf A t ->
-     elaboration G (exp_rcd l e) Inf (typ_rcd l A)  (texp_cons (stype2string  (typ_rcd l A) )  t  texp_nil) 
+     elaboration G (exp_rcd l e) Inf (typ_rcd l A)  (texp_cons (stype2string  (typ_rcd l A) )  t  texp_nil)
  | Ela_Proj : forall (G:ctx) (e:exp) (l:label) (B:typ) (t2:texp) (A:typ) (t1:texp),
      elaboration G e Inf A t1 ->
      proj t1 A l t2 B ->
@@ -592,7 +620,7 @@ Inductive elaboration : ctx -> exp -> dirflag -> typ -> texp -> Prop :=    (* de
 
 (* defns Values *)
 Inductive value : texp -> Prop :=    (* defn value *)
- | value_unit : 
+ | value_unit :
      value texp_nil
  | value_lit : forall (b:lit),
      value (texp_base b)
@@ -648,46 +676,10 @@ Inductive target_step : texp -> texp -> Prop :=    (* defn target_step *)
  | TS_AppAbs : forall (t tv:texp),
      lc_texp (texp_abs t) ->
      lc_texp tv ->
-     target_step (texp_app  (texp_abs t)  tv)  (open_texp_wrt_texp  t tv ) 
+     target_step (texp_app  (texp_abs t)  tv)  (open_texp_wrt_texp  t tv )
  | TS_Fixpoint : forall (t:texp),
      lc_texp (texp_fixpoint t) ->
      target_step (texp_fixpoint t)  (open_texp_wrt_texp  t (texp_fixpoint t) ) .
-
-(* defns RecordTypes *)
-Inductive rec_typ : ttyp -> Prop :=    (* defn rec_typ *)
- | RT_Nil : 
-     rec_typ ttyp_top
- | RT_Rcd : forall (l:label) (At Bt:ttyp),
-     rec_typ Bt ->
-     rec_typ (ttyp_rcd l At Bt).
-
-(* defns TargetEqIndexType *)
-Inductive eqIndTypTarget : ttyp -> ttyp -> Prop :=    (* defn eqIndTypTarget *)
- | TEI_top : 
-     eqIndTypTarget ttyp_top ttyp_top
- | TEI_bot : 
-     eqIndTypTarget ttyp_bot ttyp_bot
- | TEI_base : 
-     eqIndTypTarget ttyp_base ttyp_base
- | TEI_arrow : forall (At1 Bt1 At2 Bt2:ttyp),
-     eqIndTypTarget At1 At2 ->
-     eqIndTypTarget Bt1 Bt2 ->
-     eqIndTypTarget (ttyp_arrow At1 Bt1) (ttyp_arrow At2 Bt2)
- | TEI_rcd : forall (l:label) (At Ct Bt Ct' At' Bt':ttyp),
-     rec_typ Ct ->
-     rec_typ Ct' ->
-      (   (  Tlookup  l   Ct  = Some  At'   /\  eqIndTypTarget At' At )    \/   Tlookup  l   Ct  = None  )  ->
-      (   (  Tlookup  l   Ct'  = Some  Bt'   /\  eqIndTypTarget Bt' Bt )    \/   Tlookup  l   Ct'  = None  )  ->
-     eqIndTypTarget At Bt ->
-     eqIndTypTarget Ct Ct' ->
-     eqIndTypTarget (ttyp_rcd l At Ct) (ttyp_rcd l Bt Ct')
- | TEI_comm : forall (l1:label) (At:ttyp) (l2:label) (Bt Ct Ct' At' Bt':ttyp),
-     rec_typ Ct ->
-      (   (  Tlookup  l1   Ct  = Some  At'   /\  eqIndTypTarget At' At )    \/   Tlookup  l1   Ct  = None  )  ->
-      (   (  Tlookup  l2   Ct  = Some  Bt'   /\  eqIndTypTarget Bt' Bt )    \/   Tlookup  l2   Ct  = None  )  ->
-      l1  <>  l2  ->
-     eqIndTypTarget (ttyp_rcd l2 Bt  (ttyp_rcd l1 At Ct) ) Ct' ->
-     eqIndTypTarget (ttyp_rcd l1 At  (ttyp_rcd l2 Bt Ct) ) Ct'.
 
 (* defns ConcatTypes *)
 Inductive concat_typ : ttyp -> ttyp -> ttyp -> Prop :=    (* defn concat_typ *)
@@ -695,7 +687,7 @@ Inductive concat_typ : ttyp -> ttyp -> ttyp -> Prop :=    (* defn concat_typ *)
      rec_typ Bt ->
      concat_typ ttyp_top Bt Bt
  | CT_Rcd : forall (l:label) (At Bt1 Bt2 Ct At':ttyp),
-      (   (  Tlookup  l   Bt2  = Some  At'   /\  eqIndTypTarget At' At )    \/   Tlookup  l   Bt2  = None  )  ->
+      (   (  Tlookup  l   Bt2  = Some  At'   /\   subTarget  At'   At  /\ subTarget  At   At'  )    \/   Tlookup  l   Bt2  = None  )  ->
      concat_typ Bt1 Bt2 Ct ->
      concat_typ  (ttyp_rcd l At Bt1)  Bt2 (ttyp_rcd l At Ct).
 
@@ -709,17 +701,17 @@ Inductive contained_by_rec_typ : ttyp -> label -> ttyp -> Prop :=    (* defn con
 
 (* defns WelformedTypes *)
 Inductive wf_typ : ttyp -> Prop :=    (* defn wf_typ *)
- | WF_Nil : 
+ | WF_Nil :
      wf_typ ttyp_top
- | WF_Bot : 
+ | WF_Bot :
      wf_typ ttyp_bot
- | WF_Base : 
+ | WF_Base :
      wf_typ ttyp_base
  | WF_Rcd : forall (l:label) (At Bt At':ttyp),
      wf_typ At ->
      wf_typ Bt ->
      rec_typ Bt ->
-      (   (  Tlookup  l   Bt  = Some  At'   /\  eqIndTypTarget At' At )    \/   Tlookup  l   Bt  = None  )  ->
+      (   (  Tlookup  l   Bt  = Some  At'   /\   subTarget  At'   At  /\ subTarget  At   At'  )    \/   Tlookup  l   Bt  = None  )  ->
      wf_typ (ttyp_rcd l At Bt)
  | WF_Arrow : forall (At Bt:ttyp),
      wf_typ At ->
@@ -728,8 +720,8 @@ Inductive wf_typ : ttyp -> Prop :=    (* defn wf_typ *)
 
 (* defns WelformedCtx *)
 Inductive wf_ctx : tctx -> Prop :=    (* defn wf_ctx *)
- | WFC_Nil : 
-     wf_ctx  nil 
+ | WFC_Nil :
+     wf_ctx  nil
  | WFC_Cons : forall (Gt:tctx) (x:var) (At:ttyp),
      wf_typ At ->
      wf_ctx Gt ->
@@ -751,7 +743,7 @@ Inductive SubtypeTarget : ttyp -> ttyp -> Prop :=    (* defn SubtypeTarget *)
      rec_typ Ct' ->
       Tlookup  l   Ct  = Some  Bt  ->
      SubtypeTarget Bt At ->
-      (   (  Tlookup  l   Ct'  = Some  At'   /\  eqIndTypTarget At' At )    \/   Tlookup  l   Ct'  = None  )  ->
+      (   (  Tlookup  l   Ct'  = Some  At'   /\   subTarget  At'   At  /\ subTarget  At   At'  )    \/   Tlookup  l   Ct'  = None  )  ->
      SubtypeTarget Ct Ct' ->
      SubtypeTarget Ct (ttyp_rcd l At Ct').
 
@@ -771,12 +763,12 @@ Inductive target_typing : tctx -> texp -> ttyp -> Prop :=    (* defn target_typi
      target_typing Gt (texp_abs t) (ttyp_arrow At Bt)
  | TTyping_Fix : forall (L:vars) (Gt:tctx) (t:texp) (At Bt:ttyp),
       ( forall x , x \notin  L  -> target_typing  (cons ( x , Bt )  Gt )   ( open_texp_wrt_texp t (texp_var_f x) )  At )  ->
-     eqIndTypTarget At Bt ->
+      subTarget  At   Bt  /\ subTarget  Bt   At  ->
      target_typing Gt (texp_fixpoint t) At
  | TTyping_App : forall (Gt:tctx) (t1 t2:texp) (Bt At At':ttyp),
      target_typing Gt t1 (ttyp_arrow At Bt) ->
      target_typing Gt t2 At' ->
-     eqIndTypTarget At At' ->
+      subTarget  At   At'  /\ subTarget  At'   At  ->
      target_typing Gt (texp_app t1 t2) Bt
  | TTyping_RcdNil : forall (Gt:tctx),
       uniq  Gt  ->
@@ -784,10 +776,10 @@ Inductive target_typing : tctx -> texp -> ttyp -> Prop :=    (* defn target_typi
      target_typing Gt texp_nil ttyp_top
  | TTyping_RcdCons : forall (Gt:tctx) (l:label) (t1 t2:texp) (At Bt At':ttyp),
      rec_typ Bt ->
-      (   (  Tlookup  l   Bt  = Some  At'   /\  eqIndTypTarget At' At )    \/   Tlookup  l   Bt  = None  )  ->
+      (   (  Tlookup  l   Bt  = Some  At'   /\   subTarget  At'   At  /\ subTarget  At   At'  )    \/   Tlookup  l   Bt  = None  )  ->
      target_typing Gt t1 At ->
      target_typing Gt t2 Bt ->
-     target_typing Gt  (texp_cons l t1 t2)   (ttyp_rcd l At Bt) 
+     target_typing Gt  (texp_cons l t1 t2)   (ttyp_rcd l At Bt)
  | TTyping_RcdProj : forall (Gt:tctx) (t:texp) (l:label) (Bt At:ttyp),
      target_typing Gt t At ->
       Tlookup  l   At  = Some  Bt  ->
@@ -802,6 +794,4 @@ Inductive target_typing : tctx -> texp -> ttyp -> Prop :=    (* defn target_typi
 
 
 (** infrastructure *)
-Hint Constructors toplike eqIndTyp spl ord disjoint comerge cosub sub proj distapp elaboration value target_step rec_typ eqIndTypTarget concat_typ contained_by_rec_typ wf_typ wf_ctx SubtypeTarget target_typing lc_texp lc_exp : core.
-
-
+Hint Constructors toplike spl ord disjoint comerge cosub sub proj distapp elaboration value target_step rec_typ concat_typ contained_by_rec_typ wf_typ wf_ctx SubtypeTarget target_typing lc_texp lc_exp : core.
